Clean up ADT refinement, improve computation notation
The computation notation now inserts linebreaks after [;].  We also
have a tactic for rewriting with the refine monad laws.

The notion of ADT refinement now takes many fewer arguments.  In
particular, we don't need a relation between the old and new models,
just a way of doing the transformation.  The [refine]ment ensures that
we don't break anything.  The way of doing the transformation can even
be non-deterministic, though we may want to remove that feature/bug.
We may also want to make the notion of refinement proof-relevant (so
that we can extract the computation at the very end), or we may not
care, because, after all, the only thing that matters is that the
observers behave the same way.  We should probably prove an end-to-end
theorem that says that, for any initial (new) state, after any
sequence of mutation, all the observers behave the same way as they
would have in the old regime.

ADTRefinement.v
@@ -1,4 +1,4 @@
-Require Import Common Computation ADT. 
+Require Import Common Computation ADT.
 
 Generalizable All Variables.
 Set Implicit Arguments.
@@ -7,7 +7,7 @@ Set Implicit Arguments.
 Definition mutatorMethodSpec (Ty : Type) :=
   Ty    (* Initial model *)
   -> nat (* Actual argument*)
-  -> Ty (* Final Model *) 
+  -> Ty (* Final Model *)
   -> Prop.
 
 (* Specification of an observer method *)
@@ -19,160 +19,158 @@ Definition observerMethodSpec (Ty : Type) :=
 
 (** Every spec is trivially implementable using [Pick]. *)
 Section pick.
-
   Variable model : Type.
   Variable mutatorMethodIndex : Type.
   Variable observerMethodIndex : Type.
   Variable mutatorMethodSpecs : mutatorMethodIndex -> mutatorMethodSpec model.
   Variable observerMethodSpecs : observerMethodIndex -> observerMethodSpec model.
- 
+
   Definition pickImpl : ADT :=
     {|
       Model := model;
       MutatorIndex := mutatorMethodIndex;
       ObserverIndex := observerMethodIndex;
-      MutatorMethods idx := 
-        fun m x => 
-          { m' : model 
+      MutatorMethods idx :=
+        fun m x =>
+          { m' : model
           | mutatorMethodSpecs idx m x m'}%comp;
       ObserverMethods idx :=
-        fun m n => 
-          { n' : nat 
+        fun m n =>
+          { n' : nat
           | observerMethodSpecs idx m n n'}%comp
     |}.
-  
 End pick.
 
 Section MethodRefinement.
+  Variables oldModel newModel : Type.
 
-  Variables (oldModel newModel : Type). (* Old and new model *)
-  Variable absNewModel : newModel -> oldModel -> Prop.  
-  (* Abstraction relation from new to old models *)
-  
-  Variable abs : newModel -> oldModel. (* Abstraction function *)
-  Variable absValid : forall nm, absNewModel nm (abs nm). 
+  Variable abs : newModel -> Comp oldModel.
+  (** Abstraction function *)
 
-  (* Refinement of an observer method *)
-  Definition refineObserver 
-             (newObserver : observerMethodType newModel) 
-             (oldObserver : observerMethodType oldModel) :=
-      forall nm om n, 
-        absNewModel nm om -> 
-        refine (oldObserver om n) (newObserver nm n).
-  
-  (* Refinement of a mutator method *)
-  Definition refineMutator 
+  (** Refinement of a mutator method: if we first do the new
+      computation and then abstract, this is a refinement of first
+      abstracting and then doing the old computation.  That is, the
+      following diagram commutes:
+<<
+                   old mutator
+       old model --------------> old model
+          ↑                         ↑
+      abs |                         | abs
+          |                         |
+       new model --------------> new model
+                   new mutator
+>>  *)
+  Definition refineMutator
+             (oldMutator : mutatorMethodType oldModel)
              (newMutator : mutatorMethodType newModel)
-             (oldMutator : mutatorMethodType oldModel) :=
-    forall nm om n, 
-      absNewModel nm om -> 
-      forall nm', 
-        computes_to (newMutator nm n) nm' -> (* For any new mutated state *)
-          computes_to (oldMutator om n) (abs nm'). 
-  
+    := forall new_state n,
+         refine (old_state <- abs new_state;
+                 oldMutator old_state n)
+                (new_state' <- newMutator new_state n;
+                 abs new_state').
+
+  (** Refinement of an observer method: the new computation should be
+      a refinement of first abstracting and then doing the old
+      computation.  That is, the following diagram should commute:
+<<
+                  old observer
+       old model --------------> ℕ
+          ↑                      ∥
+      abs |                      ∥ id
+          |                      ∥
+       new model --------------> ℕ
+                  new observer
+>>
+   *)
+  Definition refineObserver
+             (oldObserver : observerMethodType oldModel)
+             (newObserver : observerMethodType newModel)
+    := forall new_state n,
+         refine (old_state <- abs new_state;
+                 oldObserver old_state n)
+                (newObserver new_state n).
 End MethodRefinement.
 
-Inductive refineADT : ADT -> ADT -> Prop := 
-| refinesADT : 
-    forall (oldModel newModel : Type)
-           (absNewModel : newModel -> oldModel -> Prop)
-           (abs : newModel -> oldModel) (* Abstraction function *)
-           (absValid : forall nm, absNewModel nm (abs nm)) (* absNewModel is left-total *)
-           (oldObserverMethodIndex : Type) (* Old Observer Method Index Type *)
-           (newObserverMethodIndex : Type) (* New Observer Method Index Type 
-                                             (In order to add new observers) *)
-           (mapObserverIndex : oldObserverMethodIndex -> newObserverMethodIndex)
-           (* Map from old indices to new ones *)
-           (oldMutatorMethodIndex : Type) (* Old Mutator Method Index Type *)
-           (newMutatorMethodIndex : Type) (* New Mutator Method Index Type 
-                                           (In order to add new mutators) *)
-           (mapMutatorIndex : oldMutatorMethodIndex -> newMutatorMethodIndex)
-           (* Map from old indices to new ones *)
-           (oldObserverMethods : oldObserverMethodIndex -> observerMethodType oldModel)
-           (newObserverMethods : newObserverMethodIndex -> observerMethodType newModel)
-           (oldMutatorMethods : oldMutatorMethodIndex -> mutatorMethodType oldModel)
-           (newMutatorMethods : newMutatorMethodIndex -> mutatorMethodType newModel),
-      (forall idx idx', mapObserverIndex idx = mapObserverIndex idx' -> idx = idx') -> (* mapObserverIndex is injective *)
-      (forall idx idx', mapMutatorIndex idx = mapMutatorIndex idx' -> idx = idx') -> (* mapObserverIndex is injective *)
-      (forall idx, refineObserver absNewModel (newObserverMethods (mapObserverIndex idx)) (oldObserverMethods idx)) -> 
-      (forall idx, refineMutator absNewModel abs (newMutatorMethods (mapMutatorIndex idx)) (oldMutatorMethods idx)) -> 
-      refineADT (Build_ADT newMutatorMethods newObserverMethods)
-                (Build_ADT oldMutatorMethods oldObserverMethods).
+(** We map from old indices to new indices because every method that
+    used to be callable should still be callable, and we don't care
+    about the other methods. *)
+Inductive refineADT (A B : ADT) : Prop :=
+| refinesADT :
+    forall abs mutatorMap observerMap,
+      (forall idx, @refineMutator
+                     (Model A) (Model B) abs
+                     (MutatorMethods A idx)
+                     (MutatorMethods B (mutatorMap idx)))
+      -> (forall idx, @refineObserver
+                     (Model A) (Model B) abs
+                     (ObserverMethods A idx)
+                     (ObserverMethods B (observerMap idx)))
+      -> refineADT A B.
 
-Theorem refineADT_inv old new :
-  refineADT new old -> 
-  match old with 
-    | {| Model := m;
-         MutatorIndex := mdx;
-         ObserverIndex := odx;
-         MutatorMethods := mutators;
-         ObserverMethods := observers |} => 
-      exists (absNewModel : Model new -> m -> Prop)
-             (abs : Model new -> m)
-             (mapObserverIndex : odx -> ObserverIndex new)
-             (mapMutatorIndex : mdx -> MutatorIndex new),
-        (forall nm, absNewModel nm (abs nm)) /\
-        (forall idx idx', mapObserverIndex idx = mapObserverIndex idx' -> idx = idx') /\
-      (forall idx idx', mapMutatorIndex idx = mapMutatorIndex idx' -> idx = idx') /\
-        (forall idx, refineObserver absNewModel (ObserverMethods new (mapObserverIndex idx)) (observers idx)) /\
-        (forall idx, refineMutator absNewModel abs (MutatorMethods new (mapMutatorIndex idx)) (mutators idx))
-        
-  end.
+(** We should always just unfold [refineMutator] and [refineObserver]
+    into [refine], so that we can rewrite with lemmas about [refine]. *)
+Arguments refineMutator / .
+Arguments refineObserver / .
+
+Global Instance refineADT_PreOrder : PreOrder refineADT.
 Proof.
-  destruct 1; simpl; eauto 10.
+  split; compute in *.
+  - intro x.
+    econstructor 1 with
+    (abs := @Return _)
+      (mutatorMap := id)
+      (observerMap := id);
+      unfold id; simpl; intros;
+      autorewrite with refine_monad;
+      reflexivity.
+  - intros x y z
+           [abs mutMap obsMap mutH obsH]
+           [abs' mutMap' obsMap' mutH' obsH'].
+    econstructor 1 with
+    (abs := fun z => (z' <- abs' z; abs z')%comp)
+    (mutatorMap := mutMap' ∘ mutMap)
+    (observerMap := obsMap' ∘ obsMap);
+    unfold id, compose; simpl in *; intros;
+    interleave_autorewrite_refine_monad_with setoid_rewrite_hyp.
 Qed.
 
-Section PreOrders.
+Add Parametric Relation : ADT refineADT
+  reflexivity proved by reflexivity
+  transitivity proved by transitivity
+    as refineADT_rel.
 
-  Variables (oldModel newModel : Type). (* Old and new model *)
-  Variable absNewModel : newModel -> oldModel -> Prop.  
-  Variable abs : newModel -> oldModel.
-  Variable absValid : forall nm, absNewModel nm (abs nm).
-  Variable observerMethodIndex : Type. (* Observer Method Index Type *)
-  Variable mutatorMethodIndex : Type. (* Mutator Method Index Type *)
-  Variable oldObserverMethods : observerMethodIndex -> observerMethodType oldModel.
-  Variable newObserverMethods : observerMethodIndex -> observerMethodType newModel.
-  Variable oldMutatorMethods : mutatorMethodIndex -> mutatorMethodType oldModel.
-  Variable newMutatorMethods : mutatorMethodIndex -> mutatorMethodType newModel.
+Add Parametric Morphism model mutIdx obsIdx : (@Build_ADT model mutIdx obsIdx)
+  with signature
+  (pointwise_relation _ (@refineMutator _ _ (@Return _)))
+    ==> (pointwise_relation _ (@refineObserver _ _ (@Return _)))
+    ==> refineADT
+    as refineADT_Build_ADT.
+Proof.
+  intros.
+  let A := match goal with |- refineADT ?A ?B => constr:(A) end in
+  let B := match goal with |- refineADT ?A ?B => constr:(B) end in
+  eapply (@refinesADT A B (@Return _) id id);
+    unfold id, pointwise_relation in *; simpl in *; intros;
+    auto.
+Qed.
 
-  Global Instance refineObserver_PreOrder Model : 
-    PreOrder (refineObserver (@eq Model)).
-  Proof.
-    split; compute in *; intros; subst; eauto.
-  Qed.
+(** If we had dependent setoid relations in [Type], then we could write
 
-  Add Parametric Relation Model : _ (refineObserver (@eq Model)) 
-      reflexivity proved by reflexivity
-      transitivity proved by transitivity
-    as refineObserver_rel.
+<<
+Add Parametric Morphism : @Build_ADT
+  with signature
+  (fun oldM newM => newM -> Comp oldM)
+    ==> arrow
+    ==> arrow
+    ==> (pointwise_relation _ (@refineMutator _ _ _))
+    ==> (pointwise_relation _ (@refineObserver _ _ _))
+    ==> refineADT
+    as refineADT_Build_ADT.
+Proof.
+  ...
+Qed.
+>>
 
-  Global Instance refineMutator_PreOrder Model : 
-    PreOrder (refineMutator (@eq Model) id).
-  Proof.
-    split; compute in *; intros; subst; eauto.
-  Qed.
-
-  Add Parametric Relation Model : _ (refineObserver (@eq Model)) 
-      reflexivity proved by reflexivity
-      transitivity proved by transitivity
-    as refineMutator_rel.
-
-  Global Instance refineADT_PreOrder
-  : PreOrder refineADT.
-  Proof.
-    split; compute in *.
-    intros; destruct x; econstructor 1 with 
-                        (absNewModel := @eq _)
-                          (mapObserverIndex := id)
-                          (mapMutatorIndex := id)
-                          (abs := id); eauto; reflexivity.
-    intros x y z Rxy Ryz; destruct Rxy.    
-    destruct z; inversion_by refineADT_inv.
-    econstructor 1 with (absNewModel := fun x' z => x (abs0 x') z)
-                          (mapMutatorIndex := compose mapMutatorIndex x2)
-                          (mapObserverIndex := compose mapObserverIndex x1)
-                          (abs := compose x0 abs0); 
-      eauto; compute in *; eauto.
-  Qed.
-
-End PreOrders.
+    But, alas, Matthieu is still working on those.  So the rewrite
+    machinery won't work very well when we're switching models, and
+    we'll instead have to use [etransitivity] and [apply] things. *)
